Complete implementation, soundness proof remains

AbstractInterpreter.v
@@ -1,114 +1,29 @@
-Require Import Classes.BoolType.
-Require Import Classes.Numerical.
+Require Import Classes.IsBool.
+Require Import Classes.IsNat.
 Require Import Classes.Monad.
 Require Import ConcreteInterpreter.
-Require Import Instances.BoolType.AbstractBoolean.
+Require Import Instances.Except.AbstractException.
 Require Import Instances.Galois.Parity.
+Require Import Instances.IsBool.AbstractBoolean.
+Require Import Instances.IsNat.Parity.
 Require Import Instances.Joinable.Unit.
-Require Import Instances.Numerical.Parity.
 Require Import Instances.Preorder.Unit.
+Require Import Instances.Store.AbstractStore.
 Require Import Joinable.
 Require Import Language.Statements.
 Require Import SharedInterpreter.
 Require Import Types.AbstractBool.
-Require Import Types.AbstractStore.
 Require Import Types.Maps.
 Require Import Types.Parity.
 Require Import Types.Result.
 Require Import Types.State.
+Require Import Types.Stores.
 
 Open Scope com_scope.
-
-(*Definition abstract_aexp := shared_aexp 
-  parity 
-  extract_par 
-  parity_plus 
-  parity_mult
-  abstract_store
-  get_abstract.*)
-
-  
-Definition extract (v : cvalue) : avalue :=
-  match v with
-  | VNat x => VParity (extract_par x)
-  | VBool x => VAbstrBool (extract_bool x)
-  end.
   
 Fixpoint eval_expr_abstract (e : expr) : AbstractState avalue :=
-  match e with
-  | EVal x => returnM (extract x)
-  | EVar x => st << get_abstract ;
-      returnM (st x)
-  | EPlus e1 e2 => 
-      v1 << (eval_expr_abstract e1) ;
-      v2 << (eval_expr_abstract e2) ;
-      n1 << (ensure_numerical v1) ;
-      n2 << (ensure_numerical v2) ;
-      returnM (VParity (plus_op n1 n2))
-  | EMult e1 e2 =>
-      v1 << (eval_expr_abstract e1) ;
-      v2 << (eval_expr_abstract e2) ;
-      n1 << (ensure_numerical v1) ;
-      n2 << (Numerical.ensure_numerical v2) ;
-      returnM (VParity (mult_op n1 n2))
-  | EEq e1 e2 =>
-      v1 << (eval_expr_abstract e1) ;
-      v2 << (eval_expr_abstract e2) ;
-      n1 << (ensure_numerical v1) ;
-      n2 << (ensure_numerical v2) ;
-      returnM (VAbstrBool (eq_op n1 n2))
-  | ELe e1 e2 =>
-      v1 << (eval_expr_abstract e1) ;
-      v2 << (eval_expr_abstract e2) ;
-      n1 << (ensure_numerical v1) ;
-      n2 << (ensure_numerical v2) ;
-      returnM (VAbstrBool (le_op n1 n2))
-  | ENot e =>
-      v << (eval_expr_abstract e) ;
-      b << (ensure_boolean v) ;
-      returnM (VAbstrBool (neg_op b))
-  | EAnd e1 e2 =>
-      v1 << (eval_expr_abstract e1) ;
-      v2 << (eval_expr_abstract e2) ;
-      b1 << (ensure_boolean v1) ;
-      b2 << (ensure_boolean v2) ;
-      returnM (VAbstrBool (and_op b1 b2))
-  end.
-
-Definition eval_if_abstract {A} `{Joinable A} 
-  (b : abstr_bool) (st1 st2 : AbstractState A) 
-  : AbstractState A :=
-  match b with
-  | ab_true   => st1
-  | ab_false  => st2
-  | ab_top    => join_op st1 st2
-  | ab_bottom => fail_abstract
-  end.
+  shared_eval_expr e.
   
-Definition eval_catch_abstract {A} `{Joinable A} 
-  (st1 st2 : AbstractState A) : AbstractState A :=
-  fun st => match (st1 st) with
-  | crashedA _ _ => crashedA _ _ 
-  | exceptionA _ _ st' => st2 st'
-  | exceptionOrReturn _ _ x st' => 
-      join_op (exceptionOrReturn _ _ x st') (st2 st')
-  | returnRA _ _ x st' => returnRA _ _ x st'
-  end.
 
 Fixpoint ceval_abstract (c : com) : AbstractState unit :=
-  match c with
-  | CSkip => returnM tt
-  | c1 ;c; c2 =>
-      (ceval_abstract c1) ;; (ceval_abstract c2)
-  | x ::= a => 
-      p << (eval_expr_abstract a) ;
-      st << get_abstract ;
-      put_abstract (t_update st x p)
-  | CIf b c1 c2 => 
-      v << (eval_expr_abstract b) ;
-      b' << (ensure_boolean v) ;
-      eval_if_abstract b' (ceval_abstract c1) (ceval_abstract c2)
-  | try c1 catch c2 => 
-      eval_catch_abstract (ceval_abstract c1) (ceval_abstract c2)
-  | CFail => fail_abstract
-  end.
+  shared_ceval c.
