ConcreteInterpreter.v
@@ -1,17 +1,19 @@
 Require Import Coq.Arith.Arith.
 Require Import Utf8.
 
-Require Import Classes.BoolType.
-Require Import Classes.Numerical.
+Require Import Classes.IsBool.
+Require Import Classes.IsNat.
 Require Import Classes.Monad.
-Require Import Instances.BoolType.Boolean.
-Require Import Instances.Numerical.Nat.
+Require Import Instances.Except.ConcreteException.
+Require Import Instances.IsBool.Boolean.
+Require Import Instances.IsNat.Nat.
+Require Import Instances.Store.ConcreteStore.
 Require Import Language.Statements.
 Require Import SharedInterpreter.
-Require Import Types.AbstractStore.
 Require Import Types.Maps.
 Require Import Types.Result.
 Require Import Types.State.
+Require Import Types.Stores.
 
 Open Scope com_scope.
 
@@ -24,69 +26,7 @@ Open Scope com_scope.
   get.*)
   
 Fixpoint eval_expr (e : expr) : State cvalue :=
-  match e with
-  | EVal x => returnM x
-  | EVar x => st << get ;
-      returnM (st x)
-  | EPlus e1 e2 => 
-      v1 << (eval_expr e1) ;
-      v2 << (eval_expr e2) ;
-      n1 << (ensure_numerical v1) ;
-      n2 << (ensure_numerical v2) ;
-      returnM (VNat (plus_op n1 n2))
-  | EMult e1 e2 =>
-      v1 << (eval_expr e1) ;
-      v2 << (eval_expr e2) ;
-      n1 << (ensure_numerical v1) ;
-      n2 << (ensure_numerical v2) ;
-      returnM (VNat (mult_op n1 n2))
-  | EEq e1 e2 =>
-      v1 << (eval_expr e1) ;
-      v2 << (eval_expr e2) ;
-      n1 << (ensure_numerical v1) ;
-      n2 << (ensure_numerical v2) ;
-      returnM (VBool (eq_op n1 n2))
-  | ELe e1 e2 =>
-      v1 << (eval_expr e1) ;
-      v2 << (eval_expr e2) ;
-      n1 << (ensure_numerical v1) ;
-      n2 << (ensure_numerical v2) ;
-      returnM (VBool (le_op n1 n2))
-  | ENot e =>
-      v << (eval_expr e) ;
-      b << (ensure_boolean v) ;
-      returnM (VBool (neg_op b))
-  | EAnd e1 e2 =>
-      v1 << (eval_expr e1) ;
-      v2 << (eval_expr e2) ;
-      b1 << (ensure_boolean v1) ;
-      b2 << (ensure_boolean v2) ;
-      returnM (VBool (and_op b1 b2))
-  end.
-
-Definition eval_if {A} (b : bool) (st1 st2 : State A) : State A :=
-  if b then st1 else st2.
-
-Definition eval_catch {A} (st1 st2 : State A) : State A :=
-  fun st => match (st1 st) with
-  | crashed _ _ => crashed _ _
-  | exception _ _ st' => (st2 st')
-  | x => x
-  end.
+  shared_eval_expr e.
 
 Fixpoint ceval (c : com) : State unit :=
-  match c with
-  | CSkip => returnM tt
-  | c1 ;c; c2 => 
-      (ceval c1) ;; (ceval c2)
-  | x ::= a => 
-      n << (eval_expr a) ;
-      st << get ;
-      put (t_update st x n)
-  | CIf b c1 c2 => 
-      v << (eval_expr b) ;
-      b' << (ensure_boolean v) ;
-      eval_if b' (ceval c1) (ceval c2)
-  | try c1 catch c2 => eval_catch (ceval c1) (ceval c2)
-  | CFail => fail
-  end.
+  shared_ceval c.
