SharedInterpreter.v
@@ -1,47 +1,10 @@
 Require Import Statements.
 Require Import Monad.
-(*Require Import Classes.Numerical.
-Require Import Classes.BoolType.
-Require Import Instances.Nat.Numerical.
-Require Import Instances.BoolType.Boolean.
- *)
-About nat_nat.
+Require Import Classes.IsNat.
+Require Import Classes.IsBool.
+Require Import Classes.Store.
+Require Import Classes.Except.
 
-(** MOVE ME BACK LATER *)
-Class IsBool (M : Type -> Type)
-  (valType boolType : Type) : Type :=
-{
-  ensure_bool  : valType -> M boolType;
-  build_bool   : boolType -> M valType;
-  extract_bool : bool -> M boolType;
-  and_op       : boolType -> boolType -> M boolType;
-  neg_op       : boolType -> M boolType;
-  if_op        : boolType -> M unit -> M unit -> M unit;
-}.
-
-Class IsNat (M : Type -> Type)
-  (valType boolType natType : Type) : Type :=
-{
-  ensure_nat  : valType -> M natType;
-  build_nat   : natType -> M valType;
-  extract_nat : nat -> M natType;
-  plus_op     : natType -> natType -> M natType;
-  mult_op     : natType -> natType -> M natType;
-  eq_op       : natType -> natType -> M boolType;
-  le_op       : natType -> natType -> M boolType;
-}.
-
-Class Store (M : Type -> Type) (valType : Type) :=
-{
-  get : string -> M valType
-}.
-
-Class Except (M : Type -> Type) := {
-  throw    : M unit;
-  trycatch : M unit -> M unit -> M unit;
-}.
-
-Definition admit {A} : A. Admitted.
 
 Definition extract_build_val {M : Type -> Type} {valType boolType natType : Type}
     `{Monad M, IsNat M valType boolType natType, IsBool M valType boolType}
@@ -82,78 +45,46 @@ Fixpoint shared_eval_expr
       n2 << ensure_nat v2 ;
       b << eq_op n1 n2 ;
       build_bool b
-  | _ => admit
-  end.
-
-(*
   | ELe e1 e2 =>
-      v1 << (shared_eval_expr e1) ;
-      v2 << (shared_eval_expr e2) ;
-      n1 << (ensure_nat v1) ;
-      n2 << (ensure_nat v2) ;
-      returnM (le_op n1 n2)
-  | ENot e =>
-      v << (shared_eval_expr e) ;
-      b << (BoolType.ensure_boolean v) ;
-      returnM (BoolType.neg_op b)
+      v1 << shared_eval_expr e1 ;
+      v2 << shared_eval_expr e2 ;
+      n1 << ensure_nat v1 ;
+      n2 << ensure_nat v2 ;
+      b << le_op n1 n2;
+      build_bool b
+  | ENot e1 =>
+      v1 << shared_eval_expr e1 ;
+      b1 << ensure_bool v1 ;
+      b << neg_op b1;
+      build_bool b
   | EAnd e1 e2 =>
-      v1 << (shared_eval_expr e1) ;
-      v2 << (shared_eval_expr e2) ;
-      b1 << (BoolType.ensure_boolean v1) ;
-      b2 << (BoolType.ensure_boolean v2) ;
-      returnM (BoolType.and_op b1 b2)
+      v1 << shared_eval_expr e1 ;
+      v2 << shared_eval_expr e2 ;
+      b1 << ensure_bool v1 ;
+      b2 << ensure_bool v2 ;
+      b << and_op b1 b2 ;
+      build_bool b
   end.
-*)
 
-(*Fixpoint shared_aexp 
-  {state_type : Type -> Type} 
-  `{Monad state_type}
-  (V : Type)
-  (extraction : nat -> V)
-  (plus_op mult_op : V -> V -> V)
-  (store_type : Type)
-  (getter : state_type (string -> V))
-  (e : aexp) : state_type V :=
-  match e with 
-  | ANum n => returnM (extraction n)
-  | AVar x =>
-      st << getter ;
-      returnM (st x)
-  | APlus e1 e2 =>
-      v1 << (shared_aexp V extraction plus_op mult_op store_type getter e1) ;
-      v2 << (shared_aexp V extraction plus_op mult_op store_type getter e2) ;
-      returnM (plus_op v1 v2)
-  | AMult e1 e2 =>
-      v1 << (shared_aexp V extraction plus_op mult_op store_type getter e1) ;
-      v2 << (shared_aexp V extraction plus_op mult_op store_type getter e2) ;
-      returnM (mult_op v1 v2)
+Open Scope com_scope.
+
+Fixpoint shared_ceval 
+  {M : Type -> Type} {valType natType boolType : Type}
+  `{Monad M, Store M valType, Except M, 
+    IsNat M valType boolType natType, IsBool M valType boolType}
+  (c : com) : M unit :=
+  match c with
+  | CSkip => returnM tt
+  | c1 ;c; c2 =>
+      (shared_ceval c1) ;; (shared_ceval c2)
+  | x ::= a => 
+      v << shared_eval_expr a ;
+      put x v
+  | CIf b c1 c2 => 
+      v << shared_eval_expr b ;
+      b' << ensure_bool v ;
+      if_op b' (shared_ceval c1) (shared_ceval c2)
+  | try c1 catch c2 => 
+      trycatch (shared_ceval c1) (shared_ceval c2)
+  | CFail => throw
   end.
-*)
-(*Fixpoint shared_bexp (S BV NV : Type) 
-  (extract_b : bool -> BV)
-  (extract_n : nat -> NV)
-  (equals_op : NV -> NV -> BV)
-  (le_op : NV -> NV -> BV)
-  (neg_op : BV -> BV)
-  (and_op : BV -> BV -> BV)
-  (e : bexp) :
-  State S BV :=
-  match e with
-  | BTrue => returnM (extraction true)
-  | BFalse => returnM (extraction false)
-  | BEq e1 e2 =>
-      v1 << (shared_aexp S NV extract_n equals_op le_op neg_op and_op e1) ;
-      v2 << (shared_aexp S NV extract_n equals_op le_op neg_op and_op e2) ;
-      returnM (equals_op v1 v2)
-  | BLe e1 e2 =>
-      v1 << (shared_aexp S BN NV extraction equals_op le_op neg_op and_op e1) ;
-      v2 << (shared_aexp S BN NV extraction equals_op le_op neg_op and_op e2) ;
-      returnM (le_op v1 v2)
-  | BNot b1 =>
-      v1 << (shared_bexp S BN NV extraction equals_op le_op neg_op and_op b1) ;
-      returnM (neg_op v1)
-  | BAnd b1 b2 =>
-      v1 << (shared_bexp S BN NV extraction equals_op le_op neg_op and_op b1) ;
-      v2 << (shared_bexp S BN NV extraction equals_op le_op neg_op and_op b2) ;
-      returnM (and_op v1 v2)
-  end.*)
