Classes/Except.v
@@ -1,0 +1,4 @@
+Class Except (M : Type -> Type) := {
+  throw    : M unit;
+  trycatch : M unit -> M unit -> M unit;
+}.
