Classes/Functor.v
@@ -1,0 +1,3 @@
+Class Functor (F : Type -> Type) (A B : Type) : Type := {
+  fmap : (A -> B) -> F A -> F B;
+}.
