Classes/IsBool.v
@@ -1,0 +1,10 @@
+Class IsBool (M : Type -> Type)
+  (valType boolType : Type) : Type :=
+{
+  ensure_bool  : valType -> M boolType;
+  build_bool   : boolType -> M valType;
+  extract_bool : bool -> M boolType;
+  and_op       : boolType -> boolType -> M boolType;
+  neg_op       : boolType -> M boolType;
+  if_op        : boolType -> M unit -> M unit -> M unit;
+}.
