Classes/IsNat.v
@@ -1,0 +1,11 @@
+Class IsNat (M : Type -> Type)
+  (valType boolType natType : Type) : Type :=
+{
+  ensure_nat  : valType -> M natType;
+  build_nat   : natType -> M valType;
+  extract_nat : nat -> M natType;
+  plus_op     : natType -> natType -> M natType;
+  mult_op     : natType -> natType -> M natType;
+  eq_op       : natType -> natType -> M boolType;
+  le_op       : natType -> natType -> M boolType;
+}.
