Classes/Store.v
@@ -1,0 +1,7 @@
+Require Export Coq.Strings.String.
+
+Class Store (M : Type -> Type) (valType : Type) :=
+{
+  get : string -> M valType;
+  put : string -> valType -> M unit;
+}.
