Instances/Except/AbstractException.v
@@ -1,0 +1,25 @@
+Require Import Classes.Except.
+Require Import Classes.Joinable.
+Require Import Instances.Joinable.Unit.
+Require Import Types.Stores.
+Require Import Types.Result.
+Require Import Types.State.
+
+Definition eval_catch_abstract {A} `{Joinable A} 
+  (st1 st2 : AbstractState A) : AbstractState A :=
+  fun st => match (st1 st) with
+  | crashedA _ _ => crashedA _ _ 
+  | exceptionA _ _ st' => st2 st'
+  | exceptionOrReturn _ _ x st' => 
+      join_op (exceptionOrReturn _ _ x st') (st2 st')
+  | returnRA _ _ x st' => returnRA _ _ x st'
+  end.
+
+Definition fail_abstract {A : Type} : AbstractState A :=
+  fun st => exceptionA A abstract_store st.
+
+Instance except_abstract : Except AbstractState := 
+{
+  throw := fail_abstract;
+  trycatch := eval_catch_abstract;
+}.
