Instances/Except/ConcreteException.v
@@ -1,0 +1,19 @@
+Require Import Types.State.
+Require Import Types.Result.
+Require Import Classes.Except.
+Require Import Types.Stores.
+
+Definition eval_catch {A} (st1 st2 : State A) : State A :=
+  fun st => match (st1 st) with
+  | crashed _ _ => crashed _ _
+  | exception _ _ st' => (st2 st')
+  | x => x
+  end.
+
+Definition fail {A : Type} : State A :=
+  fun st => exception A store st.
+
+Instance except_concrete : Except State := {
+  throw := fail;
+  trycatch := eval_catch;
+}.
