Instances/IsBool/AbstractBoolean.v
@@ -1,0 +1,48 @@
+Require Import Classes.IsBool.
+Require Import Classes.Joinable.
+Require Import Classes.Monad.
+Require Import Instances.Except.AbstractException.
+Require Import Instances.Joinable.Unit.
+Require Import Language.Statements.
+Require Import Types.AbstractBool.
+Require Import Types.Result.
+Require Import Types.State.
+Require Import Types.Stores.
+
+Definition ensure_abool (v : avalue) : AbstractState abstr_bool :=
+  fun st => match v with
+            | VAbstrBool b => returnRA abstr_bool abstract_store b st
+            | _ => crashedA _ _
+            end.
+
+Definition and_abM (b c : abstr_bool) := returnM (and_ab b c).
+Definition neg_abM (b : abstr_bool) := returnM (neg_ab b).
+
+Definition eval_if_abstract {A} `{Joinable A} 
+  (b : abstr_bool) (st1 st2 : AbstractState A) 
+  : AbstractState A :=
+  match b with
+  | ab_true   => st1
+  | ab_false  => st2
+  | ab_top    => join_op st1 st2
+  | ab_bottom => fail_abstract
+  end.
+
+Definition extract_ab (b : bool) : AbstractState abstr_bool := 
+  match b with
+  | true => returnM ab_true
+  | false => returnM ab_false
+  end.
+
+Definition build_abool (b : abstr_bool) : AbstractState avalue :=
+  returnM (VAbstrBool b).
+
+Instance abstract_boolean_type : IsBool AbstractState avalue abstr_bool :=
+{
+  ensure_bool := ensure_abool;
+  extract_bool := extract_ab;
+  build_bool := build_abool;
+  and_op := and_abM;
+  neg_op := neg_abM;
+  if_op := eval_if_abstract;
+}.
