Instances/IsBool/Boolean.v
@@ -1,0 +1,35 @@
+Require Import Classes.IsBool.
+Require Import Classes.Monad.
+Require Import Language.Statements.
+Require Import Types.State.
+Require Import Types.Stores.
+Require Import Types.Result.
+
+Definition ensure_bool (v : cvalue) : State bool :=
+  fun st => match v with
+            | VBool b => returnR bool store b st
+            | _ => crashed _ _
+            end.
+
+Definition build_boolean (b : bool) : State cvalue :=
+  returnM (VBool b).
+
+Definition extract_boolean (b : bool) : State bool :=
+  returnM b.
+
+Definition andbM (b c : bool) : State bool := returnM (andb b c).
+
+Definition negbM (b : bool) : State bool := returnM (negb b).
+
+Definition eval_if {A} (b : bool) (st1 st2 : State A) : State A :=
+  if b then st1 else st2.
+
+Instance boolean_type : IsBool State cvalue bool :=
+{
+  ensure_bool := ensure_bool;
+  extract_bool := extract_boolean;
+  build_bool := build_boolean;
+  and_op := andbM;
+  neg_op := negbM;
+  if_op := eval_if;
+}.
