Instances/IsNat/Nat.v
@@ -1,0 +1,35 @@
+Require Import Classes.IsNat.
+Require Import Classes.Monad.
+Require Import Types.Stores.
+Require Import Language.Statements.
+Require Import Types.State.
+Require Import Types.Result.
+
+Definition ensure_nat (v : cvalue) : State nat :=
+  fun st => match v with
+            | VNat x => returnR nat store x st
+            | _ => crashed _ _
+            end.
+
+Definition plusM (n m : nat) : State nat := returnM (plus n m).
+
+Definition multM (n m : nat) : State nat := returnM (mult n m).
+
+Definition eqbM (n m : nat) : State bool := returnM (Nat.eqb n m).
+
+Definition lebM (n m : nat) : State bool := returnM (Nat.leb n m).
+
+Definition build_natural (n : nat) : State cvalue := 
+  returnM (VNat n).
+
+Global Instance nat_numerical : IsNat State cvalue bool nat :=
+{
+  ensure_nat := ensure_nat;
+  build_nat := build_natural;
+  extract_nat := fun x => returnM x;
+  plus_op := plusM;
+  mult_op := multM;
+  eq_op := eqbM;
+  le_op := lebM;
+}.
+
