Instances/IsNat/Parity.v
@@ -1,0 +1,52 @@
+Require Import Classes.IsNat.
+Require Import Classes.Monad.
+Require Import Types.Parity.
+Require Import Types.AbstractBool.
+Require Import Language.Statements.
+Require Import Types.State.
+Require Import Types.Result.
+Require Import Types.Stores.
+
+Definition ensure_par (v : avalue) : AbstractState parity :=
+  fun st => match v with
+            | VParity x => returnRA parity abstract_store x st
+            | _ => crashedA _ _
+            end.
+
+Fixpoint extract_par (n : nat) : parity :=
+  match n with 
+  | 0 => par_even
+  | S 0 => par_odd
+  | S (S n) => extract_par n
+end.
+
+Definition extract_parM (n : nat) : AbstractState parity :=
+  returnM (extract_par n).
+
+Definition pplusM (n m : parity) : AbstractState parity :=
+  returnM (parity_plus n m).
+
+Definition pmultM (n m : parity) : AbstractState parity :=
+  returnM (parity_mult n m).
+
+Definition peqM (n m : parity) : AbstractState abstr_bool :=
+  returnM (parity_eq n m).
+
+Definition pleM (n m : parity) : AbstractState abstr_bool :=
+  returnM ab_top.
+
+Definition build_parity (p : parity) : AbstractState avalue :=
+  returnM (VParity p).
+
+Global Instance parity_numerical : 
+  IsNat AbstractState avalue abstr_bool parity :=
+{
+  ensure_nat := ensure_par;
+  extract_nat := extract_parM;
+  build_nat := build_parity;
+  plus_op := pplusM;
+  mult_op := pmultM;
+  eq_op := peqM;
+  le_op := pleM;
+}.
+
