Instances/Store/AbstractStore.v
@@ -1,0 +1,29 @@
+Require Export Coq.Strings.String.
+Require Import Classes.Store.
+Require Import Language.Statements.
+Require Import Types.Maps.
+Require Import Types.Result.
+Require Import Types.State.
+Require Import Types.Stores.
+
+Definition abstract_store_top : abstract_store :=
+  fun _ => VTop.
+Definition abstract_store_bottom : abstract_store :=
+  fun _ => VBottom.
+Definition abstract_store_join
+    (ast1 ast2 : abstract_store) : abstract_store :=
+  fun x => VTop.
+
+Definition abstract_store_get (x : string) : 
+  AbstractState avalue := 
+  fun st => returnRA avalue abstract_store (st x) st.
+
+Definition abstract_store_put 
+  (x : string) (v : avalue) : 
+  AbstractState unit :=
+  fun st => returnRA unit abstract_store tt st.
+
+Instance store_abstract : Store AbstractState avalue := {
+  get := abstract_store_get;
+  put := abstract_store_put;
+}.
