Instances/Store/ConcreteStore.v
@@ -1,0 +1,20 @@
+Require Import Types.Maps.
+Require Import Language.Statements.
+Require Import Classes.Store.
+Require Import Types.State.
+Require Import Types.Result.
+Require Import Types.Stores.
+
+Definition store_get (x : string) : State cvalue := fun st =>
+  returnR cvalue store (st x) st.
+
+Definition store_put (x : string) (v : cvalue) : State unit := 
+  fun st => returnR unit store tt st.
+
+Check store_put.
+Check put.
+
+Instance store_concrete : Store State cvalue := {
+  get := store_get;
+  put := store_put;
+}.
