Types/Stores.v
@@ -1,0 +1,5 @@
+Require Import Types.Maps.
+Require Import Language.Statements.
+
+Definition abstract_store := total_map avalue.
+Definition store := total_map cvalue.
